Utils/SetExt.dfy
@@ -11,4 +11,27 @@ module SetExt {
   //  if |xs| == 1 then xs[0] else Math.Max(xs[0], Max(xs[1..]))
   //}
 
+    ghost function ToSeq<T>(s: set<T>): (r: seq<T>)
+        ensures |s| == |r|
+    {
+        if |s| == 0 then
+            []
+        else
+            var y :| y in s;
+            var r := s - {y};
+            [y] + ToSeq(r)
+    }
+
+    lemma ToSeqStillContains<T>(s: set<T>, x: T)
+        requires x in s
+        ensures x in ToSeq(s)
+    {
+    }
+
+    function SetProduct<T, U>(t: set<T>, u: set<U>): (r: set<(T, U)>)
+    {
+        (set x: T, y: U | x in t && y in u :: (x, y))
+    }
+
+
 }
