Test/Primitives.dfy
@@ -36,7 +36,7 @@ module Primitives {
     const xor_port_bound: C.CPort := 3
 
     lemma nk_xor_valid()
-        ensures C.CNodeKindValid(0, xor_port_bound, nk_xor)
+        ensures C.CNodeKindValid(0, nk_xor)
     {
     }
 
